Splinter/Journal/ReprJournalRefinement.i.dfy
@@ -1,0 +1,114 @@
+include "ReprJournal.i.dfy"
+include "LinkedJournalRefinement.i.dfy"
+
+module ReprJournalRefinement {
+  import opened ReprJournal
+  import LinkedJournal
+  import LinkedJournalRefinement
+
+// PROVE INVARIANTS
+
+  predicate Inv(v: Variables)
+  {
+    && v.WF()
+    && v.journal.truncatedJournal.diskView.Acyclic()
+    // && v.journal.truncatedJournal.RepresentationIsTight(v.reprIndex.Values)
+  }
+
+  lemma InvNext(v: Variables, v': Variables, lbl: TransitionLabel)
+    requires Inv(v)
+    requires Next(v, v', lbl)
+    ensures Inv(v')
+  {
+    var step: Step :| NextStep(v, v', lbl, step);
+    match step {
+      case ReadForRecoveryStep(depth) => {
+        assert LinkedJournal.NextStep(v.journal, v'.journal, lbl, step);
+        LinkedJournalRefinement.InvNext(v.journal, v'.journal, lbl);
+        assert Inv(v');
+      }
+      case FreezeForCommitStep(depth) => {
+        assert LinkedJournal.NextStep(v.journal, v'.journal, lbl, step);
+        LinkedJournalRefinement.InvNext(v.journal, v'.journal, lbl);
+        assert Inv(v');
+      } 
+      case ObserveFreshJournalStep() => {
+        assert LinkedJournal.NextStep(v.journal, v'.journal, lbl, step);
+        LinkedJournalRefinement.InvNext(v.journal, v'.journal, lbl);
+        assert Inv(v');
+      } 
+      case PutStep() => {
+        assert LinkedJournal.NextStep(v.journal, v'.journal, lbl, step);
+        LinkedJournalRefinement.InvNext(v.journal, v'.journal, lbl);
+        assert Inv(v');
+      }
+      case DiscardOldStep() => {
+        // TODO
+        assume LinkedJournal.NextStep(v.journal, v'.journal, lbl, step);
+        LinkedJournalRefinement.InvNext(v.journal, v'.journal, lbl);
+        assert Inv(v');
+      }
+      case InternalJournalMarshalStep(cut) => {
+        assert LinkedJournal.NextStep(v.journal, v'.journal, lbl, step);
+        LinkedJournalRefinement.InvNext(v.journal, v'.journal, lbl);
+        assert Inv(v');
+      }
+    }
+  }
+
+
+// PROVE REFINEMENT
+
+  function I(v: Variables) : (out: LinkedJournal.Variables) 
+  {
+    v.journal
+  }
+
+  lemma InitRefines(v: Variables, tj: TruncatedJournal)
+    requires Init(v, tj)
+    ensures LinkedJournal.Init(I(v), tj)
+  {}
+
+  lemma DiscardOldStepRefines(v: Variables, v': Variables, lbl: TransitionLabel, step: Step)
+    requires Inv(v)
+    requires Inv(v')
+    requires NextStep(v, v', lbl, step)
+    requires step.DiscardOldStep?
+    ensures LinkedJournal.DiscardOld(I(v), I(v'), lbl)
+  {
+
+    assert LinkedJournal.DiscardOld(I(v), I(v'), lbl);
+  }
+
+  lemma NextRefines(v: Variables, v': Variables, lbl: TransitionLabel)
+    requires Inv(v)
+    requires Next(v, v', lbl)
+    ensures v'.WF()
+    ensures Inv(v')
+    ensures LinkedJournal.Next(I(v), I(v'), lbl)
+  {
+    InvNext(v, v', lbl);
+    var step: Step :| NextStep(v, v', lbl, step);
+    match step {
+      case ReadForRecoveryStep(depth) => {
+        assert LinkedJournal.NextStep(I(v), I(v'), lbl, step);
+      }
+      case FreezeForCommitStep(depth) => {
+        assert LinkedJournal.NextStep(I(v), I(v'), lbl, step);
+      } 
+      case ObserveFreshJournalStep() => {
+        assert LinkedJournal.NextStep(I(v), I(v'), lbl, step);
+      } 
+      case PutStep() => {
+        assert LinkedJournal.NextStep(I(v), I(v'), lbl, step);
+      }
+      case DiscardOldStep() => {
+        DiscardOldStepRefines(v, v', lbl, step);
+        assert LinkedJournal.NextStep(I(v), I(v'), lbl, step);
+      }
+      case InternalJournalMarshalStep(cut) => {
+        assert LinkedJournal.NextStep(I(v), I(v'), lbl, step);
+      }
+    }
+  }
+}
